Absolutely! Here's how to solve the problem:

**1. Find the First Derivative, y':**

* Use the chain rule: 
   * The derivative of the outside function (e^u) is e^u.
   * The derivative of the inside function (3x^2) is 6x.

* Putting it together:
   y' = (1/6) * e^(3x^2) * 6x = x * e^(3x^2)

**2. Find the Second Derivative, y":**

* Use the product rule:
   * (uv)' = u'v + uv'

* Let u = x and v = e^(3x^2)
   * u' = 1
   * v' = 6x * e^(3x^2) (from the first derivative)

* Putting it together:
   y" = (1 * e^(3x^2)) + (x * 6x * e^(3x^2))
   y" = e^(3x^2) + 6x^2 * e^(3x^2)

**3. Evaluate y"(0):**

* Substitute x = 0 into the second derivative:
   y"(0) = e^(3*0^2) + 6(0)^2 * e^(3*0^2)
   y"(0) = e^0 + 0
   y"(0) = 1

**Answer:**

The answer is **B**.
