Let's go through each part of the question step-by-step.

### (a) Find the slope of the line tangent to the graph of \( f \) at \( x = \pi \).

The function \( f(x) = \cos(2x) + e^{\sin(x)} \) is given. To find the slope of the tangent line at \( x = \pi \), we need to compute \( f'(\pi) \).

The derivative of \( f(x) \), \( f'(x) \), is calculated as follows:
- The derivative of \( \cos(2x) \) is \( -2\sin(2x) \) using the chain rule.
- The derivative of \( e^{\sin(x)} \) is \( e^{\sin(x)} \cos(x) \) using the chain rule.

Thus,
\[ f'(x) = -2\sin(2x) + e^{\sin(x)}\cos(x) \]

Substitute \( x = \pi \) into the derivative:
\[ f'(\pi) = -2\sin(2\pi) + e^{\sin(\pi)}\cos(\pi) \]
\[ f'(\pi) = -2(0) + e^0(-1) \]
\[ f'(\pi) = -1 \]

So, the slope of the tangent line at \( x = \pi \) is \(-1\).

### (b) Find \( k'(\pi) \), where \( k(x) = h(f(x)) \).

To find \( k'(x) \), we use the chain rule:
\[ k'(x) = h'(f(x)) \cdot f'(x) \]

Given \( h(x) \) is the function shown in the graph, we need \( h'(x) \) and \( f(x) \) at \( x = \pi \).

1. **Calculate \( f(\pi) \):**
   \[ f(\pi) = \cos(2\pi) + e^{\sin(\pi)} \]
   \[ f(\pi) = 1 + 1 = 2 \]

2. **Find \( h'(2) \):** 
   From the graph, the derivative \( h'(x) \) at \( x = 2 \) can be found by the slope of the line segment at that point. The slope \( h'(x) \) from \( x = 1 \) to \( x = 2 \) is \( \frac{0 - 1}{2 - 1} = -1 \).

3. **Calculate \( k'(\pi) \):**
   \[ k'(\pi) = h'(f(\pi)) \cdot f'(\pi) \]
   \[ k'(\pi) = h'(2) \cdot (-1) \]
   \[ k'(\pi) = (-1)(-1) = 1 \]

So, \( k'(\pi) = 1 \).

### (c) Find \( m'(2) \), where \( m(x) = g(-2x) \cdot h(x) \).

To find \( m'(x) \), we use the product rule:
\[ m'(x) = g'(-2x)(-2)h(x) + g(-2x)h'(x) \]

Substitute \( x = 2 \):
1. **Calculate \( g(-4) \) and \( g'(-4) \) using the table:**
   - \( g(-4) = 5 \)
   - \( g'(-4) = -1 \)

2. **Calculate \( h(2) \) and \( h'(2) \):**
   - From the graph, \( h(2) = 1 \)
   - \( h'(2) = -1 \) as calculated earlier.

Thus,
\[ m'(2) = (-1)(-2)(1) + (5)(-1) \]
\[ m'(2) = 2 - 5 \]
\[ m'(2) = -3 \]

So, \( m'(2) = -3 \).

### (d) Is there a number \( c \) in the closed interval \([-5, -3]\) such that \( g'(c) = -4 \)?

Looking at the table, \( g' \) takes values from -3 to 4. Since \( g'(-5) = -3 \) and \( g'(-3) = 4 \), and \( -4 \) is not explicitly listed in the table, we use the Intermediate Value Theorem (IVT). The IVT states that if a function is continuous on a closed interval \([a, b]\) and \( N \) is between \( f(a) \) and \( f(b) \), then there exists a \( c \) in \((a, b)\) such that \( f(c) = N \).

Since \( g' \) is continuous (as \( g \) is differentiable), and \( g' \) changes from \(-3\) to \(4\) between \( -5 \) and \( -3 \), there must be some \( c \) in \([-5, -3]\) such that \( g'(c) = -4 \).

Hence, by IVT, there exists such a number \( c \) in the interval \([-5, -3]\).
