Absolutely! Here's how to solve the problem using implicit differentiation:

**1. Implicit Differentiation**

We'll differentiate both sides of the equation with respect to 'x', remembering to treat 'y' as a function of 'x':

* d/dx (2x^4) - d/dx (xy) + d/dx (3y^3) = d/dx (12)

* 8x^3 - [1*y + x*(dy/dx)] + 9y^2 (dy/dx) = 0

**2. Isolate dy/dx**

Our goal is to solve for dy/dx:

* 8x^3 - y - x(dy/dx) + 9y^2 (dy/dx) = 0
* (dy/dx) (9y^2 - x) = y - 8x^3
* dy/dx = (y - 8x^3) / (9y^2 - x)

**Answer:**

The answer is **C**.
